lib/concurrency: initial progress on update for env monad
These are experimental changes to the refinement framework and are still
being iterated on. Most proofs have not been updated yet and are broken,
although minimal changes have been made to avoid any getting completely
stuck.

Signed-off-by: Corey Lewis <corey.lewis@proofcraft.systems>

lib/concurrency/Prefix_Refinement.thy
@@ -26,7 +26,9 @@ text \<open>
 text \<open>
   Fragments must be self-closed, or enabled. Certain incomplete traces
   must be possible to extend by a program step.\<close>
-definition self_closed :: "((tmid \<times> 's) list \<Rightarrow> bool) \<Rightarrow> 's \<Rightarrow> ('s, 'a) tmonad \<Rightarrow> bool" where
+definition self_closed ::
+  "((tmid \<times> 's) list \<Rightarrow> bool) \<Rightarrow> ('c, 's) monad_state \<Rightarrow> ('c, 's, 'a) tmonad \<Rightarrow> bool"
+  where
   "self_closed cond s f =
      (\<forall>xs. (xs, Incomplete) \<in> f s \<longrightarrow> cond xs \<longrightarrow> (\<exists>s'. (Me, s') # xs \<in> fst ` f s))"
 
@@ -36,7 +38,9 @@ text \<open>
   Fragments must be environment-closed. Certain incomplete traces
   must be possible to extend by any environment step that is
   compatible with some condition.\<close>
-definition env_closed :: "((tmid \<times> 's) list \<Rightarrow> 's \<Rightarrow> bool) \<Rightarrow> 's \<Rightarrow> ('s, 'a) tmonad \<Rightarrow> bool" where
+definition env_closed ::
+  "((tmid \<times> 's) list \<Rightarrow> 's \<Rightarrow> bool) \<Rightarrow> ('c, 's) monad_state \<Rightarrow> ('c, 's, 'a) tmonad \<Rightarrow> bool"
+  where
   "env_closed cond s f =
      (\<forall>xs s'. (xs, Incomplete) \<in> f s \<longrightarrow> cond xs s' \<longrightarrow> ((Env, s') # xs) \<in> fst ` f s)"
 
@@ -46,9 +50,15 @@ lemma env_closed_strengthen_cond:
   "\<lbrakk>env_closed P s f; \<forall>xs s. Q xs s \<longrightarrow> P xs s\<rbrakk> \<Longrightarrow> env_closed Q s f"
   by (simp add: env_closed_def)
 
+text \<open>@{text mrel} type: @{typ "('c, 's) monad_state"} state relations\<close>
+type_synonym ('c, 's, 'd, 't) mrel = "('c, 's) monad_state \<Rightarrow> ('d, 't) monad_state \<Rightarrow> bool"
+
 text \<open>Two traces match according to some state relation if they match at every step.\<close>
-definition matching_tr :: "('s \<Rightarrow> 't \<Rightarrow> bool) \<Rightarrow> (tmid \<times> 's) list \<Rightarrow> (tmid \<times> 't) list \<Rightarrow> bool" where
-  "matching_tr sr = list_all2 (\<lambda>(aid, as) (cid, cs). aid = cid \<and> sr as cs)"
+definition matching_tr ::
+  "('s \<Rightarrow> 't \<Rightarrow> bool) \<Rightarrow> (tmid \<times> 's) list \<Rightarrow> (tmid \<times> 't) list \<Rightarrow> bool"
+  where
+  "matching_tr sr =
+     list_all2 (\<lambda>(aid, as) (cid, cs). aid = cid \<and> sr as cs)"
 
 definition matching_tr_pfx ::
   "('s \<Rightarrow> 't \<Rightarrow> bool) \<Rightarrow> (tmid \<times> 's) list \<Rightarrow> (tmid \<times> 't) list \<Rightarrow> bool"
@@ -63,8 +73,24 @@ abbreviation (input)
   "matching_self_cond ctr \<equiv> (\<lambda>xs. length xs < length ctr \<and> fst (rev ctr ! length xs) = Me)"
 
 abbreviation (input)
-  "matching_env_cond sr ctr s0 R \<equiv>
-     (\<lambda>xs s. matching_tr_pfx sr ((Env, s) # xs) ctr \<and> rely_cond R s0 ((Env, s) # xs))"
+  "matching_env_cond sr ctr c s0 R \<equiv>
+     (\<lambda>xs s. matching_tr_pfx sr ((Env, s) # xs) ctr \<and> rely_cond R c s0 ((Env, s) # xs))"
+
+abbreviation with_env_sr :: "('c, 's, 'd, 't) mrel \<Rightarrow> 'c \<Rightarrow> 'd \<Rightarrow> 's \<Rightarrow> 't \<Rightarrow> bool" where
+  "with_env_sr R c d s t \<equiv> R (monad_state c s) (monad_state d t)"
+
+abbreviation with_env_of_sr ::
+  "('c, 's, 'd, 't) mrel \<Rightarrow> ('c, 's) monad_state \<Rightarrow> ('d, 't) monad_state \<Rightarrow> 's \<Rightarrow> 't \<Rightarrow> bool"
+  where
+  "with_env_of_sr R s t \<equiv> with_env_sr R (env s) (env t)"
+
+abbreviation with_env_R :: "('c, 's) rg_pred \<Rightarrow> 'c \<Rightarrow> 's \<Rightarrow> 's \<Rightarrow> bool" where
+  "with_env_R R c \<equiv> with_env_sr R c c"
+
+abbreviation with_env_of_R ::
+  "('c, 's) rg_pred \<Rightarrow> ('c, 's) monad_state \<Rightarrow> 's \<Rightarrow> 's \<Rightarrow> bool"
+  where
+  "with_env_of_R R s \<equiv> with_env_of_sr R s s"
 
 text \<open>
   The collection of properties a fragment must have to match some concrete
@@ -73,18 +99,18 @@ text \<open>
   the rely condition, the concrete trace (or a prefix), and must either be
   a matching result or @{term Incomplete} if a prefix.\<close>
 definition is_matching_fragment ::
-  "('s \<Rightarrow> 't \<Rightarrow> bool) \<Rightarrow> ('s \<Rightarrow> 't \<Rightarrow> bool) \<Rightarrow> ('a \<Rightarrow> 'b \<Rightarrow> bool) \<Rightarrow> (tmid \<times> 't) list \<Rightarrow>
-   ('t, 'b) tmres \<Rightarrow> 's \<Rightarrow> ('s \<Rightarrow> 's \<Rightarrow> bool) \<Rightarrow> 's \<Rightarrow> ('s, 'a) tmonad \<Rightarrow> bool"
+  "('c, 's, 'd, 't) mrel \<Rightarrow> ('c, 's, 'd, 't) mrel \<Rightarrow> ('a \<Rightarrow> 'b \<Rightarrow> bool) \<Rightarrow> 'd \<Rightarrow> (tmid \<times> 't) list \<Rightarrow>
+   ('t, 'b) tmres \<Rightarrow> 's \<Rightarrow> ('c, 's) rg_pred \<Rightarrow> ('c, 's) monad_state \<Rightarrow> ('c, 's, 'a) tmonad \<Rightarrow> bool"
   where
-  "is_matching_fragment sr osr rvr ctr cres s0 R s f
+  "is_matching_fragment sr osr rvr c' ctr cres s0 R s f
      = ((prefix_closed f
          \<and> self_closed (matching_self_cond ctr) s f
-         \<and> env_closed (matching_env_cond sr ctr s0 R) s f)
+         \<and> env_closed (matching_env_cond (with_env_sr sr (env s) c') ctr (env s) s0 R) s f)
         \<and> f s \<noteq> {}
-        \<and> (\<forall>(tr, res) \<in> f s. rely_cond R s0 tr
-             \<and> matching_tr_pfx sr tr ctr
+        \<and> (\<forall>(tr, res) \<in> f s. rely_cond R (env s) s0 tr
+             \<and> matching_tr_pfx (with_env_sr sr (env s) c') tr ctr
              \<and> (length tr < length ctr \<longrightarrow> res = Incomplete)
-             \<and> (length tr = length ctr \<longrightarrow> rel_tmres osr rvr res cres)))"
+             \<and> (length tr = length ctr \<longrightarrow> rel_tmres (with_env_sr osr (env s) c') rvr res cres)))"
 
 lemmas is_matching_fragmentD = is_matching_fragment_def[THEN iffD1, rule_format]
 
@@ -106,15 +132,15 @@ text \<open>
 \<comment> \<open>FIXME: should we have an option for showing non-failure of the concrete program.\<close>
 \<comment> \<open>FIXME: corres uses a set for the state relation, this uses a predicate. Do we care?\<close>
 definition prefix_refinement ::
-  "('s \<Rightarrow> 't \<Rightarrow> bool) \<Rightarrow> ('s \<Rightarrow> 't \<Rightarrow> bool) \<Rightarrow> ('s \<Rightarrow> 't \<Rightarrow> bool) \<Rightarrow> ('a \<Rightarrow> 'b \<Rightarrow> bool) \<Rightarrow>
-   ('s \<Rightarrow> 's \<Rightarrow> bool) \<Rightarrow> ('t \<Rightarrow> 't \<Rightarrow> bool) \<Rightarrow> ('s \<Rightarrow> 's \<Rightarrow> bool) \<Rightarrow> ('t \<Rightarrow> 't \<Rightarrow> bool) \<Rightarrow>
-   ('s, 'a) tmonad \<Rightarrow> ('t, 'b) tmonad \<Rightarrow> bool"
+  "('c, 's, 'd, 't) mrel \<Rightarrow> ('c, 's, 'd, 't) mrel \<Rightarrow> ('c, 's, 'd, 't) mrel \<Rightarrow> ('a \<Rightarrow> 'b \<Rightarrow> bool) \<Rightarrow>
+   ('c, 's) rg_pred \<Rightarrow> ('d, 't) rg_pred \<Rightarrow> ('c, 's) m2_pred \<Rightarrow> ('d, 't) m2_pred \<Rightarrow>
+   ('c, 's, 'a) tmonad \<Rightarrow> ('d, 't, 'b) tmonad \<Rightarrow> bool"
   where
   "prefix_refinement sr isr osr rvr AR R P Q aprog cprog
-    = (\<forall>s s0 t0 t. isr s t \<longrightarrow> P s0 s \<longrightarrow> sr s0 t0 \<longrightarrow> Q t0 t
+    = (\<forall>s s0 t0 t. isr s t \<longrightarrow> P (with_env_of s s0) s \<longrightarrow> with_env_of_sr sr s t s0 t0 \<longrightarrow> Q (with_env_of t t0) t
          \<longrightarrow> (\<forall>(ctr, cres) \<in> cprog t.
-                rely_cond R t0 ctr \<longrightarrow>
-                  (\<exists>f. is_matching_fragment sr osr rvr ctr cres s0 AR s f
+                rely_cond R (env t) t0 ctr \<longrightarrow>
+                  (\<exists>f. is_matching_fragment sr osr rvr (env t) ctr cres s0 AR s f
                        \<and> triv_refinement aprog f)))"
 
 abbreviation
@@ -146,18 +172,18 @@ lemma matching_tr_pfx_aCons:
   done
 
 lemma rely_cond_hd:
-  "\<lbrakk>rely_cond R s0 xs; xs \<noteq> []\<rbrakk>
-   \<Longrightarrow> fst (hd xs) = Env \<longrightarrow> R (last_st_tr (tl xs) s0) (snd (hd xs))"
+  "\<lbrakk>rely_cond R c s0 xs; xs \<noteq> []\<rbrakk>
+   \<Longrightarrow> fst (hd xs) = Env \<longrightarrow> R (monad_state c (last_st_tr (tl xs) s0)) (monad_state c (snd (hd xs)))"
   by (clarsimp simp: rely_cond_def neq_Nil_conv trace_steps_append
               split: if_split_asm)
 
 lemma rely_cond_nth:
-  "\<lbrakk>rely_cond R s0 tr; n < length tr\<rbrakk>
-   \<Longrightarrow> fst (rev tr ! n) = Env \<longrightarrow> R ((if n = 0 then s0 else snd (rev tr ! (n - 1)))) (snd (rev tr ! n))"
+  "\<lbrakk>rely_cond R c s0 tr; n < length tr\<rbrakk>
+   \<Longrightarrow> fst (rev tr ! n) = Env \<longrightarrow> R (monad_state c ((if n = 0 then s0 else snd (rev tr ! (n - 1))))) (monad_state c (snd (rev tr ! n)))"
   by (simp add: rely_cond_def trace_steps_rev_drop_nth[where n=0, simplified])
 
 lemma is_matching_fragment_Nil:
-  "is_matching_fragment sr osr rvr ctr cres s0 R s f \<Longrightarrow> [] \<in> fst ` f s"
+  "is_matching_fragment sr osr rvr c' ctr cres s0 R s f \<Longrightarrow> [] \<in> fst ` f s"
   apply (clarsimp simp: is_matching_fragment_def)
   apply (clarsimp simp only: set_eq_iff empty_iff simp_thms not_all)
   apply (drule(1) prefix_closed_drop[where tr=tr and n="length tr" for tr])
@@ -193,16 +219,16 @@ lemma prefix_refinement_serial:
   oops\<close>
 
 lemma is_matching_fragment_no_trace:
-  "is_matching_fragment sr osr rvr [] cres s0 R s (\<lambda>s. {([], ares s)})
-   = rel_tmres osr rvr (ares s) cres"
+  "is_matching_fragment sr osr rvr c' [] cres s0 R s (\<lambda>s. {([], ares s)})
+   = rel_tmres (with_env_sr osr (env s) c') rvr (ares s) cres"
   by (simp add: is_matching_fragment_def prefix_closed_def self_closed_def env_closed_def
                 matching_tr_pfx_def matching_tr_def)
 
 \<comment> \<open>Singleton trace monads must have an empty trace to be prefix_closed\<close>
 lemma prefix_refinement_singleton:
   "prefix_refinement sr isr osr rvr AR R P Q (\<lambda>s. {([], res s)}) (\<lambda>s. {([], cres s)})
-   = (\<forall>s0 s t0 t. isr s t \<longrightarrow> P s0 s \<longrightarrow> sr s0 t0 \<longrightarrow> Q t0 t
-          \<longrightarrow> rel_tmres osr rvr (res s) (cres t))"
+   = (\<forall>s0 s t0 t. isr s t \<longrightarrow> P (with_env_of s s0) s \<longrightarrow> with_env_of_sr sr s t s0 t0 \<longrightarrow> Q (with_env_of t t0) t
+          \<longrightarrow> rel_tmres (with_env_of_sr osr s t) rvr (res s) (cres t))"
   (is "prefix_refinement _ _ _ _ _ _ _ _ ?f _ = _")
   apply (rule iffI; clarsimp simp: prefix_refinement_def)
    apply ((drule spec)+, (drule (1) mp)+)
@@ -223,8 +249,8 @@ lemma prefix_refinement_singleton:
 lemma prefix_refinement_no_trace:
   "no_trace g
    \<Longrightarrow> prefix_refinement sr isr osr rvr AR R P Q f g
-       = (\<forall>s0 s t0 t. isr s t \<longrightarrow> P s0 s \<longrightarrow> sr s0 t0 \<longrightarrow> Q t0 t
-            \<longrightarrow> (\<forall>cres \<in> snd ` (g t). \<exists>(tr, res) \<in> (f s). tr = [] \<and> rel_tmres osr rvr res cres))"
+       = (\<forall>s0 s t0 t. isr s t \<longrightarrow> P (with_env_of s s0) s \<longrightarrow> with_env_of_sr sr s t s0 t0 \<longrightarrow> Q (with_env_of t t0) t
+            \<longrightarrow> (\<forall>cres \<in> snd ` (g t). \<exists>(tr, res) \<in> (f s). tr = [] \<and> rel_tmres (with_env_of_sr osr s t) rvr res cres))"
   apply (rule iffI; clarsimp simp: prefix_refinement_def; drule (1) no_traceD; clarsimp)
    apply ((drule spec)+, (drule (1) mp)+)
    apply (drule (1) bspec, clarsimp)
@@ -244,8 +270,8 @@ lemma prefix_refinement_no_trace:
 
 lemma prefix_refinement_no_trace':
   "\<lbrakk>no_trace g;
-    \<And>s0 s t0 t. \<lbrakk>isr s t; P s0 s; sr s0 t0; Q t0 t\<rbrakk>
-                \<Longrightarrow> (\<forall>cres \<in> snd ` (g t). \<exists>(tr, res) \<in> (f s). tr = [] \<and> rel_tmres osr rvr res cres)\<rbrakk>
+    \<And>s0 s t0 t. \<lbrakk>isr s t; P (with_env_of s s0) s; with_env_of_sr sr s t s0 t0; Q (with_env_of t t0) t\<rbrakk>
+                \<Longrightarrow> (\<forall>cres \<in> snd ` (g t). \<exists>(tr, res) \<in> (f s). tr = [] \<and> rel_tmres (with_env_of_sr osr s t) rvr res cres)\<rbrakk>
    \<Longrightarrow> prefix_refinement sr isr osr rvr AR R P Q f g"
   by (simp add: prefix_refinement_no_trace)
 
@@ -253,17 +279,17 @@ section \<open>Building blocks\<close>
 text \<open>Prefix refinement rules for basic constructs.\<close>
 
 lemma default_prefix_refinement_ex:
-  "is_matching_fragment sr osr rvr ctr cres s0 R s
+  "is_matching_fragment sr osr rvr c' ctr cres s0 R s
      (\<lambda>s. aprog s \<inter> ({tr'. length tr' \<le> length ctr} \<times> UNIV))
-   \<Longrightarrow> \<exists>f. is_matching_fragment sr osr rvr ctr cres s0 R s f \<and> triv_refinement aprog f"
+   \<Longrightarrow> \<exists>f. is_matching_fragment sr osr rvr c' ctr cres s0 R s f \<and> triv_refinement aprog f"
   apply (intro exI conjI, assumption)
   apply (simp add: triv_refinement_def)
   done
 
 lemma default_prefix_refinement_ex_match_iosr_R:
-  "is_matching_fragment sr osr rvr ctr cres s0 R s
+  "is_matching_fragment sr osr rvr c' ctr cres s0 R s
      (rely (\<lambda>s. aprog s \<inter> ({tr'. matching_tr_pfx iosr tr' ctr} \<times> UNIV)) R s0)
-   \<Longrightarrow> \<exists>f. is_matching_fragment sr osr rvr ctr cres s0 R s f \<and> triv_refinement aprog f"
+   \<Longrightarrow> \<exists>f. is_matching_fragment sr osr rvr c' ctr cres s0 R s f \<and> triv_refinement aprog f"
   apply (intro exI conjI, assumption)
   apply (clarsimp simp: triv_refinement_def rely_def)
   done
@@ -309,13 +335,13 @@ text \<open>
   allow us to prove the existence of a matching trace in the abstract
   program.\<close>
 theorem matching_fragment_matching_tr:
-  assumes match: "is_matching_fragment sr osr rvr ctr cres s0 R' s f"
-  and rely: "rely_cond R t0 ctr"
-  and sr0: "sr s0 t0"
-  and sr: "(\<forall>s t t'. sr s t \<longrightarrow> R t t' \<longrightarrow> (\<exists>s'. sr s' t' \<and> R' s s'))"
-  shows "\<exists>(atr, ares) \<in> f s. matching_tr sr atr ctr
-                    \<and> rel_tmres osr rvr ares cres
-                    \<and> rely_cond R' s0 atr"
+  assumes match: "is_matching_fragment sr osr rvr c' ctr cres s0 R' s f"
+  and rely: "rely_cond R c' t0 ctr"
+  and sr0: "with_env_sr sr (env s) c' s0 t0"
+  and sr: "\<forall>s t t'. sr s t \<longrightarrow> R t t' \<longrightarrow> (\<exists>s'. sr s' t' \<and> R' s s')"
+  shows "\<exists>(atr, ares) \<in> f s. matching_tr (with_env_sr sr (env s) c') atr ctr
+                    \<and> rel_tmres (with_env_sr osr (env s) c') rvr ares cres
+                    \<and> rely_cond R' (env s) s0 atr"
 proof -
 
   note pfx_closed = is_matching_fragment_prefix_closed[OF match]
@@ -326,43 +352,38 @@ proof -
   note pfx_closedD = pfx_closed[THEN prefix_closedD]
 
   have extend:
-    "\<And>tmid s' tr res. ((tmid, s') # tr, res) \<in> f s \<Longrightarrow> rely_cond R' s0 tr
-        \<Longrightarrow> \<exists>x res. (x # tr, res) \<in> f s \<and> rely_cond R' s0 (x # tr)"
+    "\<And>tmid s' tr res. ((tmid, s') # tr, res) \<in> f s \<Longrightarrow> rely_cond R' (env s) s0 tr
+        \<Longrightarrow> \<exists>x res. (x # tr, res) \<in> f s \<and> rely_cond R' (env s) s0 (x # tr)"
     apply (case_tac tmid)
      apply (fastforce simp: rely_cond_Cons)
     apply (frule f_prop[OF pfx_closedD], clarsimp)
     apply (frule f_prop, clarsimp simp: matching_tr_pfx_aCons)
     apply (frule rely_cond_nth[rotated], rule rely, simp)
-    apply (drule_tac s="last_st_tr tr s0" in sr[rule_format, rotated])
+    apply (drule_tac s="with_env_of s (last_st_tr tr s0)" in sr[rule_format, rotated])
      apply (clarsimp simp: sr0 neq_Nil_conv matching_tr_pfx_aCons)
-    apply clarsimp
-    apply (rename_tac t' s'_rely)
-    apply (drule_tac s'="s'_rely" in env_closedD[where f=f, OF env_closed, OF prefix_closedD[OF pfx_closed]])
-     apply (clarsimp simp: matching_tr_pfx_aCons rely_cond_Cons_eq)
-    apply clarsimp
-    apply (fastforce intro!: rely_cond_Cons)
+    apply fastforce
     done
 
   have extend2:
-    "\<And>tr res. (tr, res) \<in> f s \<Longrightarrow> rely_cond R' s0 tr
+    "\<And>tr res. (tr, res) \<in> f s \<Longrightarrow> rely_cond R' (env s) s0 tr
         \<Longrightarrow> length tr < length ctr
-        \<Longrightarrow> \<exists>x res. (x # tr, res) \<in> f s \<and> rely_cond R' s0 (x # tr)"
+        \<Longrightarrow> \<exists>x res. (x # tr, res) \<in> f s \<and> rely_cond R' (env s) s0 (x # tr)"
     apply (frule f_prop, clarsimp)
     apply (case_tac "fst (rev ctr ! length tr)")
      apply (frule self_closed[THEN self_closedD], simp)
      apply (fastforce intro: rely_cond_Cons)
     apply (frule rely_cond_nth[rotated], rule rely, simp)
-    apply (drule_tac s="last_st_tr tr s0" in sr[rule_format, rotated])
+    apply (drule_tac s="with_env_of s (last_st_tr tr s0)" in sr[rule_format, rotated])
      apply (clarsimp simp: sr0 neq_Nil_conv matching_tr_pfx_aCons)
     apply clarsimp
-    apply (drule_tac s'=s' in env_closedD[OF env_closed])
+    apply (drule_tac s'="mstate s'" in env_closedD[OF env_closed])
      apply (simp add: matching_tr_pfx_aCons prod_eq_iff rely_cond_Cons)
     apply (fastforce intro: rely_cond_Cons)
     done
 
   { fix n
     have "\<exists>(tr, res) \<in> f s. (n \<le> length ctr \<longrightarrow> length tr = n)
-        \<and> rely_cond R' s0 tr"
+        \<and> rely_cond R' (env s) s0 tr"
       apply (induct n)
        apply (cut_tac f=f in is_matching_fragment_Nil;
           (rule sr0 match)?)
@@ -388,7 +409,7 @@ qed
 
 corollary matching_fragment_matching_tr_trivR:
   assumes match: "is_matching_fragment sr osr rvr ctr cres s0 R s f"
-  and sr: "(\<forall>s t t'. sr s t \<longrightarrow> (\<exists>s'. sr s' t' \<and> R s s'))"
+  and sr: "(\<forall>s' t' t''. sr s' t' \<longrightarrow> (\<exists>s''. sr s'' t'' \<and> with_env_R R (env s) s' s''))"
   and srx: "sr s0 t0"
   shows "\<exists>(atr, ares) \<in> f s. matching_tr sr atr ctr \<and> rel_tmres osr rvr ares cres"
   using matching_fragment_matching_tr[where R="\<lambda>_ _. True", OF match _ srx]
@@ -397,14 +418,14 @@ corollary matching_fragment_matching_tr_trivR:
 theorem prefix_refinement_rely_cond_trD:
   assumes preds: "prefix_refinement sr isr osr rvr AR R P Q aprog cprog"
     "isr s t" "P s0 s" "Q t0 t" "(ctr, cres) \<in> cprog t"
-    "rely_cond R t0 ctr" "sr s0 t0"
+    "rely_cond R (env t) t0 ctr" "sr (with_env_of s s0) (with_env_of t t0)"
   and sr: "(\<forall>s t t'. sr s t \<longrightarrow> R t t' \<longrightarrow> (\<exists>s'. sr s' t' \<and> AR s s'))"
-  shows "\<exists>(atr, ares) \<in> aprog s. matching_tr sr atr ctr
-                    \<and> rel_tmres osr rvr ares cres
-                    \<and> rely_cond AR s0 atr"
+  shows "\<exists>(atr, ares) \<in> aprog s. matching_tr (with_env_of_sr sr s t) atr ctr
+                    \<and> rel_tmres (with_env_of_sr osr s t) rvr ares cres
+                    \<and> rely_cond AR (env s) s0 atr"
 proof -
   obtain f where subs: "f s \<subseteq> aprog s"
-      and match: "is_matching_fragment sr osr rvr ctr cres s0 AR s f"
+      and match: "is_matching_fragment (with_env_of_sr sr s t) (with_env_of_sr osr s t) rvr ctr cres s0 AR s f"
     using prefix_refinementD[OF preds(1-3) _ preds(4-5)] preds(6-)
     by (auto simp add: triv_refinement_def)
   show ?thesis
@@ -626,8 +647,8 @@ lemma ball_set_zip_conv_nth:
   "(\<forall>x \<in> set (zip ys zs). P x) = (\<forall>n. n < length ys \<longrightarrow> n < length zs \<longrightarrow> P (ys ! n, zs ! n))"
   by (auto simp: Ball_def in_set_zip)
 
-definition par_tr_fin_principle :: "('s, unit) tmonad \<Rightarrow> bool" where
-  "par_tr_fin_principle f = (\<forall>s tr s'. (tr, Result ((), s')) \<in> f s \<longrightarrow> s' = last_st_tr tr s \<and> tr \<noteq> [])"
+definition par_tr_fin_principle :: "('c, 's, unit) tmonad \<Rightarrow> bool" where
+  "par_tr_fin_principle f = (\<forall>s tr s'. (tr, Result ((), s')) \<in> f s \<longrightarrow> s' = last_st_tr tr (mstate s) \<and> tr \<noteq> [])"
 
 lemmas par_tr_fin_principleD = par_tr_fin_principle_def[THEN iffD1, rule_format]
 
@@ -697,7 +718,7 @@ lemma par_tr_fragment_parallel_def:
 
 lemmas list_all2_rev_nthD = list_all2_nthD[OF list_all2_rev[THEN iffD2], simplified]
 
-definition forward_enabled :: "'s rg_pred \<Rightarrow> bool" where
+definition forward_enabled :: "('c, 's) rg_pred \<Rightarrow> bool" where
   "forward_enabled P = (\<forall>s_pre. \<exists>s. P s_pre s)"
 
 lemmas forward_enabledD = forward_enabled_def[THEN iffD1, rule_format]
@@ -939,13 +960,13 @@ lemma is_matching_fragment_UNION:
   This is a variant of @{term Trace_Monad.bind}, that is used to build up the fragment required
   for proving @{text prefix_refinement_bind_general}.\<close>
 definition mbind ::
-  "('s, 'a) tmonad \<Rightarrow> ('s \<Rightarrow> 'a \<Rightarrow> ('s, 'b) tmonad) \<Rightarrow> 's \<Rightarrow> ('s, 'b) tmonad"
+  "('c, 's, 'a) tmonad \<Rightarrow> ('s \<Rightarrow> 'a \<Rightarrow> ('c, 's, 'b) tmonad) \<Rightarrow> 's \<Rightarrow> ('c, 's, 'b) tmonad"
   where
   "mbind f g s0 \<equiv> \<lambda>s. \<Union>(xs, r) \<in> (f s).
      case r of
          Failed \<Rightarrow> {(xs, Failed)}
        | Incomplete \<Rightarrow> {(xs, Incomplete)}
-       | Result (rv, s) \<Rightarrow> fst_upd (\<lambda>ys. ys @ xs) ` g (last_st_tr xs s0) rv s"
+       | Result (rv, s') \<Rightarrow> fst_upd (\<lambda>ys. ys @ xs) ` g (last_st_tr xs s0) rv (with_env_of s s')"
 
 lemma self_closed_mbind:
   "\<lbrakk>is_matching_fragment sr osr rvr ctr cres s0 R s f;
@@ -1529,6 +1550,7 @@ lemma prefix_refinement_noop2:
   apply (insert nf)
   apply (clarsimp simp: no_trace_def no_fail_def failed_def image_def)
   apply (subgoal_tac "\<exists>(r, s')\<in>mres (f s). rel_tmres iosr dc (Result (r, s')) b")
+sorry
    apply (case_tac b; fastforce simp: mres_def intro: rev_bexI)
   apply (rule use_exs_valid)
    apply (rule exs_hoare_post_imp[rotated])
@@ -2033,20 +2055,20 @@ lemma whenM_prefix_refinement:
   done
 
 
-section \<open>prefix_refinement rules for env_step, commit_step, interference and await\<close>
+section \<open>prefix_refinement rules for env_step, commit_step, interference and Await\<close>
 \<comment> \<open>FIXME: better name for section\<close>
 
 lemma Int_insert_left2:
   "(insert a B \<inter> C) = ((if a \<in> C then {a} else {}) \<union> (B \<inter> C))"
   by auto
 
-definition rely_stable :: "('t \<Rightarrow> 't \<Rightarrow> bool) \<Rightarrow> ('s \<Rightarrow> 't \<Rightarrow> bool) \<Rightarrow> ('t \<Rightarrow> bool) \<Rightarrow> bool" where
+definition rely_stable :: "('d, 't) rg_pred \<Rightarrow> ('c, 's, 'd, 't) mrel \<Rightarrow> ('d, 't) mpred \<Rightarrow> bool" where
   "rely_stable R sr Q = (\<forall>s t t'. Q t \<and> sr s t \<and> R t t' \<longrightarrow> Q t' \<and> (\<exists>s'. sr s' t'))"
 
 lemmas rely_stableD = rely_stable_def[THEN iffD1, simplified imp_conjL, rule_format]
 
 definition env_rely_stable_iosr ::
-  "'s rg_pred \<Rightarrow> 't rg_pred \<Rightarrow> ('s \<Rightarrow> 't \<Rightarrow> bool) \<Rightarrow> ('s \<Rightarrow> 't \<Rightarrow> bool) \<Rightarrow> ('t \<Rightarrow> bool) \<Rightarrow> bool"
+  "('c, 's) rg_pred \<Rightarrow> ('d, 't) rg_pred \<Rightarrow> ('c, 's, 'd, 't) mrel \<Rightarrow> ('c, 's, 'd, 't) mrel \<Rightarrow> ('d, 't) mpred \<Rightarrow> bool"
   where
   "env_rely_stable_iosr AR R sr iosr Q =
      (\<forall>s0 t0 s t. Q t0 \<longrightarrow> iosr s0 t0 \<longrightarrow> R t0 t \<longrightarrow> AR s0 s \<longrightarrow> sr s t \<longrightarrow> iosr s t)"
@@ -2054,7 +2076,7 @@ definition env_rely_stable_iosr ::
 lemmas env_rely_stable_iosrD = env_rely_stable_iosr_def[THEN iffD1, rule_format]
 
 definition env_stable ::
-  "'s rg_pred \<Rightarrow> 't rg_pred \<Rightarrow> ('s \<Rightarrow> 't \<Rightarrow> bool) \<Rightarrow> ('s \<Rightarrow> 't \<Rightarrow> bool) \<Rightarrow> ('t \<Rightarrow> bool) \<Rightarrow> bool"
+  "('c, 's) rg_pred \<Rightarrow> ('d, 't) rg_pred \<Rightarrow> ('c, 's, 'd, 't) mrel \<Rightarrow> ('c, 's, 'd, 't) mrel \<Rightarrow> ('d, 't) mpred \<Rightarrow> bool"
   where
   "env_stable AR R sr iosr Q = (rely_stable R sr Q \<and> env_rely_stable_iosr AR R sr iosr Q \<and> iosr \<le> sr)"
 
@@ -2110,6 +2132,7 @@ proof -
            simp add: prefix_closed_def in_fst_snd_image_eq self_closed_def
                      matching_tr_pfx_def matching_tr_def
                      env_closed_def)
+sorry
      apply (metis env_rely_stable_iosrD[OF est])
     apply clarsimp
     apply (auto dest: rely_stableD[OF st] predicate2D[OF sr])[1]
@@ -2212,7 +2235,7 @@ lemma prefix_refinement_interference:
   apply (clarsimp simp: guar_cond_def)
   done
 
-lemma prefix_refinement_await:
+lemma prefix_refinement_Await:
   "\<lbrakk>env_stable AR R sr iosr Q; abs_rely_stable AR P;
     \<forall>s t. P s \<longrightarrow> Q t \<longrightarrow> iosr s t \<longrightarrow> G' t \<longrightarrow> G s;
     (\<exists>s. G' s) \<longrightarrow> (\<exists>s. G s)\<rbrakk>
@@ -2410,6 +2433,7 @@ lemma prefix_refinement_in_place_trans:
     apply (clarsimp simp: is_matching_fragment_def)
    apply (drule(2) matching_fragment_matching_tr, simp)
    apply (clarsimp simp: matching_tr_def dest!: list_all2_lengthD)
+sorry
    apply blast
   apply (clarsimp simp: triv_refinement_def)
   apply blast
